\documentclass[../main.tex]{subfiles}
\begin{document}
	\chapter{Binomial Theorem}
	For a binomial expansion $(a+b)^n$, there are $(n+1)$ terms and $(a+b+c)^n$ has $\dfrac{(n+1)(n+2)}{2}$ terms.
	\section{Expansion of a binomial expression}
	\begin{align}
				(a+b)^n & = ^nC_0 a^n b^0 + ^nC_1 a^{n-1} b^1 + ^nC_2 a^{n-2} b^2 + \cdots + ^nC_n a^0 b^n \nonumber \\
				& = \sum_{i=0}^{n} {^nC_{i}} a^{n-i} b^i \nonumber \\
				& \forall n \in \mathbb{N}\\				
				(a+b)^n & = a^n b^0 + na^{n-1} b + \dfrac{n(n-1)}{2!} a^{n-2} b^2  + \cdots + \dfrac{n(n-1) \cdots 3 \cdot 2 \cdot 1}{n!} a^0 b^n + \cdots \infty \nonumber\\
				&\forall n \in \mathbb{R}
	\end{align}
	
	\section{Trinomial Expansion}
	For $(a+b+c)^n$:
	\begin{align}
		(a+b+c+)^n = \sum \dfrac{n!}{i! j! k!} a^i b^j c^k \nonumber\\
		\forall (i+j+k) = n \text{; } i,j,k,n \in \mathbb{N}
	\end{align}
	
	\section{Properties of Coefficients}
	\begin{align}
		&\text{Sum of Co-efficients: } C_0 + C_1 + C_2 + \cdots + C_{n-1} + C_n = 2^n\\
		&\text{Sum of Odd Co-efficients: } C_0 + C_2 + C_4 + \cdots + C_{2n-3} + C_{2n-1} = 2^{n-1}\\
		& C_0 - C_1 + C_2 - \cdots + C_{2n-1} - C_{2n} = 0
	\end{align}
	
	\section{Pascal's Rule}
	For $1 \leq k \leq n$ and  $k,n \in \mathbb{N}$:
	\begin{align}
		{{n}\choose{k}} + {{n}\choose{k-1}} = {{n+1}\choose{k}} 
	\end{align}
\end{document}