\documentclass[../main.tex]{subfiles}

\begin{document}
	\chapter{Logarithm}	\pagenumbering{roman}
	\section{Basic Formulae}
	For $a^x=b$:
	\begin{align}
		& \log_{a}{x}, \forall x \leq 0 \text{ is undefined}\\
		& \log_a b = x, bax \neq 1, a \neq 1\\
		& \log_b a^m = m \log_b a \text{, for } a^m=b\\
		& a^{\log_a x} = x\\
		& a^{\log_b c} = c^{\log_b a}\\
		& \frac{1}{\log_a b} = \log_b a\\
		& \log_c (ab) = \log_c a+\log_c b\\
		& \log_c \left( \frac{a}{b} \right) = \log_c a-\log_c b\\
		& \vert \log_a x \vert=\begin{cases}
			-\log_a x, \text{ if } \, 0 < x < 1\\
			\log_a x, \text{ if } \, 1\leq x < \infty \\
		\end{cases}
	\end{align}
	
	\section{Series}
	\begin{align}
		& e^x = 1 + \frac{x}{1!} + \frac{x^2}{2!} + \frac{x^3}{3!} + \cdots \infty = \lim_{n \to \infty} \sum_{i=0}^{n} \frac{x^i}{i!} \\
		& \log(1+x) = x - \frac{x^2}{2} + \frac{x^3}{3} - \frac{x^4}{4} + \cdots \infty = \lim_{n\to\infty} \sum_{i=1}^{n}(-1)^{(i-1)} \frac{x^i}{i}
	\end{align}
\end{document}