\documentclass[../main.tex]{subfile}
\begin{document}
    \chapter{Reduction Formula}
    \section{Circular Trigonometric Functions}
        \begin{align}
            \int \sin^n x dx & = -\dfrac{1}{n} \sin^{n-1} x \cos x dx + \dfrac{n-1}{n} \int \sin^{n - 2} x dx \\
            \int \cos^n x dx & = -\dfrac{1}{n} \cos^{n-1} x \sin x dx + \dfrac{n-1}{n} \int \cos^{n-2} x dx \\
            \int_0^{\frac{\pi}{2}} \sin^n x dx & = \int_0^{ \frac{\pi}{2} } \cos^n x dx =
                \begin{cases}
                    \dfrac{(n-1)\cdot(n-3)\cdots 3\cdot1}{n\cdot(n-2)\cdots 4\cdot 2}\left(\dfrac{\pi}{2}\right), n\rightarrow \text{even}\\
                    \dfrac{(n-1)\cdot(n-3)\cdots 4\cdot2}{n\cdot(n-2)\cdots 3\cdot 1}, n\rightarrow \text{odd}
                \end{cases}\\
            \int \sin^m x \cos^n x dx & = \dfrac{-\sin^{m - 1} x \cos^{n + 1} x}{m + n} + \dfrac{m - 1}{m + n} \int \sin^{m-2} x \cos^n x dx
        \end{align}
        
        \section{Special Definite Integrations}
        For $I(m,n)=\int_0^{\frac{\pi}{2}} \sin^m x\cos^n x dx$:
        \begin{align}
            I(m,n) & = \dfrac{[(m - 1) \cdot (m - 3) \cdots 3 \cdot 1][(n - 1) \cdot (n - 3) \cdots 3 \cdot 1]}{(m + n) \cdot (m + n - 1) \cdots (4) \cdot (2)} \cdot \dfrac{\pi}{2} \rightarrow m,n \text{ are even}\\
            I(m,n) & = \dfrac{[(m - 1) \cdot (m - 3) \cdots (2\text{ or }1)][(n - 1) \cdot (n-3) \cdots (2\text{ or }1)]}{(m + n) \cdot (m + n - 1) \cdots (2\text{ or }1)} \rightarrow \text{ all other cases}\\
        \end{align}

        \section{Recursive Forms in Circular Trigonometric Functions}
        \begin{align}
            I_n & = \int \tan^n x dx\nonumber\\
            \Rightarrow I_n & = \dfrac{\tan^{n - 2} x}{n - 1} - I_{n-2}\\
            \hline
            I_n & = \int \cot^n x dx \nonumber\\
            \Rightarrow I_n & = - \dfrac{\cot^{n - 2} x}{n - 1} - I_{n - 2}\\
            \hline
            I_n & = \int \sec^n x dx \nonumber\\
            \Rightarrow I_n & = \dfrac{\sec^{n - 2} x \tan x}{n - 1} + \dfrac{n - 2}{n - 1} I_{n-2}\\
            \hline
            I_n & = \int \csc^n x dx \nonumber\\
            \Rightarrow I_n & = -\dfrac{ \csc^{n - 2} x \cot x }{ n - 1 } + \dfrac{ n - 2 }{ n - 1 } I_{ n - 2 }\\
            \hline
            I_n & = \int x^n e^{ax} dx\\
            \int x^n e^{ax} dx & = \dfrac{x^n e^{ax}}{a} - \dfrac{n}{a} I_{n-2}\\
            \hline
            I(m,n) & = \int x^m (\ln x)^n dx\\
            \int x^m (\ln x)^n dx & = \dfrac{x^{m + 1}}{m + 1}(\ln x)^n - \dfrac{n}{m + 1} I_{m,n-1}
        \end{align}
\end{document}